Source/DafnyCore/AST/Statements/Assignment/UpdateStmt.cs
@@ -128,16 +128,7 @@ public class UpdateStmt : ConcreteUpdateStatement, ICloneable<UpdateStmt>, ICanR
     }
 
     // resolve proof
-    if (Proof != null) {
-      // clear the labels for the duration of checking the proof body, because break statements are not allowed to leave the proof body
-      var prevLblStmts = resolver.EnclosingStatementLabels;
-      var prevLoopStack = resolver.LoopStack;
-      resolver.EnclosingStatementLabels = new Scope<Statement>(resolver.Options);
-      resolver.LoopStack = new List<Statement>();
-      resolver.ResolveStatement(Proof, resolutionContext);
-      resolver.EnclosingStatementLabels = prevLblStmts;
-      resolver.LoopStack = prevLoopStack;
-    }
+    resolver.ResolveByProof(Proof, resolutionContext);
 
     // figure out what kind of UpdateStmt this is
     if (firstEffectfulRhs == null) {
