Source/IntegrationTests/TestFiles/LitTests/LitTest/dafny0/CallBy.dfy
@@ -1,28 +1,6 @@
 // RUN: %testDafnyForEachResolver --expect-exit-code=4 "%s" -- --standard-libraries
 
-datatype Option<+T> = None | Some(value: T) {
-  function UnwrapOr(default: T): T {
-    match this
-    case Some(v) => v
-    case None() => default
-  }
-
-  predicate IsFailure() {
-    None?
-  }
-
-  function PropagateFailure<U>(): Option<U>
-    requires None?
-  {
-    None
-  }
-
-  function Extract(): T
-    requires Some?
-  {
-    value
-  }
-}
+import opened Std.Wrappers
 
 opaque predicate P() { true }
 
@@ -30,46 +8,51 @@ lemma ProveP() ensures P() {
   reveal P();
 }
 
-method M()
+method NeedsP()
   requires P()
 {}
 
-method M'() returns (r: int)
+method NeedsPAndReturns3() returns (r: int)
   requires P()
   ensures r == 3
 { r := 3; }
 
-method M''() returns (r: Option<int>)
+method NeedsPAndReturnsNone() returns (r: Option<int>)
   requires P()
 { r := None; }
 
 method A() {
-  M() by { ProveP(); }
+  NeedsP() by { ProveP(); }
   assert P(); // Should fail
 }
 
 method B() {
   var v: int;
-  v := M'() by { reveal P(); }
+  v := NeedsPAndReturns3() by { reveal P(); }
   assert P(); // Should fail
 }
 
 method C() {
   assert p: P() by { ProveP(); }
-  var v' := M'() by { reveal p; }
-  assert v' == 3;  // should pass
+  var v := NeedsPAndReturns3() by { reveal p; }
+  assert v == 3;  // should pass
   assert P(); // should fail
 }
 
 method D() returns (r: Option<int>){
   var v: int;
-  v :- M''() by { ProveP(); }
+  v :- NeedsPAndReturnsNone() by {
+    match false {
+      case true => assert true;
+      case false => ProveP();
+    }
+  }
   assert P(); // should fail
   r := None;
 }
 
 method E() returns (r: Option<int>){
-  var v' :- M''() by { reveal P(); }
+  var v :- NeedsPAndReturnsNone() by { reveal P(); }
   assert P(); //  should fail
   r := None;
 }
